theories/Decidability/Soundness.v
@@ -1,9 +1,9 @@
 (** * LogRel.Decidability.Soundness: the implementations imply the inductive predicates. *)
-From Coq Require Import Nat Lia Arith.
+From Coq Require Import Nat List Lia Arith ssrbool.
 From Equations Require Import Equations.
 From LogRel.AutoSubst Require Import core unscoped Ast Extra.
 From LogRel Require Import Utils BasicAst Context Notations UntypedReduction DeclarativeTyping DeclarativeInstance GenericTyping NormalForms.
-From LogRel Require Import Validity LogicalRelation Fundamental DeclarativeSubst TypeConstructorsInj AlgorithmicTyping BundledAlgorithmicTyping Normalisation.
+From LogRel Require Import Validity LogicalRelation Fundamental DeclarativeSubst TypeConstructorsInj AlgorithmicTyping BundledAlgorithmicTyping Normalisation TypeUniqueness.
 From LogRel.Decidability Require Import Functions.
 From PartialFun Require Import Monad PartialFun.
 
@@ -12,7 +12,236 @@ Import IndexedDefinitions.
 
 Set Universe Polymorphism.
 
-Section RedImplemSound.
+Definition well_typed_stack Γ A t B (π : stack) :=
+  forall u, [Γ |- t ≅ u : A] -> [Γ |- (zip u π) : B].
+
+Lemma well_typed_stack_conv_in Γ A A' t B (π : stack) :
+  well_typed_stack Γ A t B π ->
+  [Γ |- A ≅ A'] ->
+  well_typed_stack Γ A' t B π.
+Proof.
+  unfold well_typed_stack.
+  intros Hπ Hconv u Hu.
+  eapply Hπ.
+  now econstructor.
+Qed.
+
+Lemma well_typed_zip Γ B t π :
+  [Γ |- zip t π : B] ->
+  ∑ A, [Γ |- t : A] × well_typed_stack Γ A t B π.
+Proof.
+intros Hty.
+induction π as [|[]] in t, B, Hty |- * ; cbn.
+- exists B ; split.
+  1: eassumption.
+  intros u ** ; cbn.
+  boundary.
+- unfold well_typed_stack in * ; cbn in *.
+  eapply IHπ in Hty as (T&(?&[]&?)%termGen'&Hstack) ; subst.
+  eexists ; split ; tea.
+  intros u Htyu.
+  eapply Hstack.
+  econstructor.
+  1: eapply TermEmptyElimCong ; tea ; refold.
+  2: eassumption.
+  now econstructor.
+- unfold well_typed_stack in * ; cbn in *.
+  eapply IHπ in Hty as (T&(?&[]&?)%termGen'&Hstack) ; subst.
+  eexists ; split ; tea.
+  intros u Htyu.
+  eapply Hstack.
+  econstructor.
+  1: eapply TermNatElimCong ; tea ; refold.
+  + now econstructor.
+  + now econstructor.
+  + now eapply TermRefl.
+  + eassumption.
+- unfold well_typed_stack in * ; cbn in *.
+  eapply IHπ in Hty as (T&(?&(?&?&[])&?)%termGen'&Hstack) ; subst.
+  eexists ; split ; tea.
+  intros u' Htyu.
+  eapply Hstack.
+  econstructor.
+  1: econstructor ; tea.
+  2: eassumption.
+  now econstructor.
+- unfold well_typed_stack in * ; cbn in *.
+  eapply IHπ in Hty as [T [[?[[?[?[->]]]]]%termGen' Hstack]].
+  eexists; split; tea.
+  intros; eapply Hstack.
+  eapply TermConv; refold; tea.
+  now econstructor.
+- unfold well_typed_stack in * ; cbn in *.
+  eapply IHπ in Hty as [T [[?[[?[?[->]]]]]%termGen' Hstack]].
+  eexists; split; tea.
+  intros; eapply Hstack.
+  eapply TermConv; refold; tea.
+  now econstructor.
+- unfold well_typed_stack in * ; cbn in *.
+  eapply IHπ in Hty as [T [[?[[]]]%termGen' Hstack]]; subst.
+  eexists; split; tea.
+  intros; eapply Hstack.
+  eapply TermConv; refold; tea.
+  econstructor; tea; now (eapply TypeRefl + eapply TermRefl).
+Qed.
+
+Lemma zip_app t π π' : zip t (π ++ π') = zip (zip t π) π'.
+Proof.
+  induction π in t |- * ; cbn ; eauto.
+Qed.
+
+(* Lemma compact_app t π π' : compact t (π ++ π') = compact (compact t π) π'.
+Proof.
+  induction π in t |- * ; cbn ; eauto.
+Qed. *)
+
+Lemma well_typed_zip_app Γ A t B π π' :
+  [Γ |- t : A] ->
+  well_typed_stack Γ A t B (π ++ π') ->
+  ∑ T, well_typed_stack Γ A t T π × well_typed_stack Γ T (zip t π) B π'.
+Proof.
+  intros Ht Hπ.
+  unshelve epose proof (Hπ t _) as Hzip.
+  1: now econstructor.
+  rewrite zip_app in Hzip.
+  eapply well_typed_zip in Hzip as [T [Hzip]].
+  eapply well_typed_zip in Hzip as [A' []].
+  eexists ; split ; tea.
+  eapply well_typed_stack_conv_in ; tea.
+  now eapply typing_unique.
+Qed.
+
+Corollary well_typed_zip_cons Γ A t B s π :
+  [Γ |- t : A] ->
+  well_typed_stack Γ A t B (s :: π) ->
+  ∑ T, [Γ |- zip1 t s : T] × well_typed_stack Γ T (zip1 t s) B π.
+Proof.
+  intros Ht Hty.
+  change (s :: π) with ([:: s] ++ π) in Hty.
+  eapply well_typed_zip_app in Hty as [? [Hts]] ; tea.
+  cbn in *.
+  eexists ; split ; tea.
+  eapply Hts.
+  now econstructor.
+Qed.
+
+(* Definition nomap_stack π :=
+  forallb (fun s => match s with | eMap _ _ _ => false | _ => true end) π.
+
+Definition ismap_stack π :=
+  forallb (fun s => match s with | eMap _ _ _ => true | _ => false end) π.
+
+Lemma stack_ne n π :
+  nomap_stack π -> whne n -> whne (zip n π).
+Proof.
+  intros Hπ Hne.
+  induction π as [|[]] in n, Hne, Hπ |- * ; cbn.
+  1: eassumption.
+  1-5: cbn in * ; eapply IHπ ; tea ; now econstructor.
+  cbn in * ; congruence.
+Qed. *)
+
+(* Lemma stack_compact_nomap n π :
+  whne n -> nomap_stack π -> compact n π = zip n π.
+Proof.
+  intros Hne Hπ.
+  induction π as [|[] π] in n, Hne, Hπ |- * ; cbn in * ; try fold (nomap_stack π) in Hπ.
+  1: reflexivity.
+  1-5: eapply IHπ ; tea ; now econstructor.
+  now congruence.
+Qed.
+
+Lemma stack_compact_map n π :
+  ismap_stack π -> whne_list n -> whne_list (compact n π).
+Proof.
+  intros Hπ Hne.
+  induction π as [|[]] in n, Hne, Hπ |- * ; cbn.
+  1: eassumption.
+  1-5: cbn in * ; congruence.
+  destruct (Map.into_view n) ; cbn in *.
+  - eapply IHπ ; tea.
+    econstructor.
+    inversion Hne ; subst ; tea.
+    exfalso ; now inversion H.
+  - eapply IHπ ; tea.
+    econstructor.
+    inversion Hne ; subst ; tea.
+    cbn in *.
+    now congruence.
+Qed. *)
+
+(* Lemma list_stack_ismap Γ A t B (π : stack) :
+  [Γ |- t : tList A] ->
+  well_typed_stack Γ (tList A) t B π ->
+  ismap_stack π.
+Proof.
+  intros Ht Hπ.
+  induction π as [|[] π] in A, t, B, Ht, Hπ |- * ; cbn.
+  - easy.
+  - eapply well_typed_zip_cons in Hπ as [? [(?&[[-> ? Ht']])%termGen']] ; subst ; tea.
+    unshelve eapply typing_unique, ty_conv_inj in Ht ; last first ; tea.
+    2-3: now econstructor.
+    now cbn in *.
+  - eapply well_typed_zip_cons in Hπ as [? [(?&[[-> ? Ht']])%termGen']] ; subst ; tea.
+    unshelve eapply typing_unique, ty_conv_inj in Ht ; last first ; tea.
+    2-3: now econstructor.
+    now cbn in *.
+  - eapply well_typed_zip_cons in Hπ as [? [(?&[(?&?&[->])])%termGen']] ; subst ; tea.
+    unshelve eapply typing_unique, ty_conv_inj in Ht ; last first ; tea.
+    2-3: now econstructor.
+    now cbn in *.
+  - eapply well_typed_zip_cons in Hπ as [? [(?&[(?&?&[->])])%termGen']] ; subst ; tea.
+    unshelve eapply typing_unique, ty_conv_inj in Ht ; last first ; tea.
+    2-3: now econstructor.
+    now cbn in *.
+  - eapply well_typed_zip_cons in Hπ as [? [(?&[(?&?&[->])])%termGen']] ; subst ; tea.
+    unshelve eapply typing_unique, ty_conv_inj in Ht ; last first ; tea.
+    2-3: now econstructor.
+    now cbn in *.
+  - eapply well_typed_zip_cons in Hπ as [? [[? [[] Hconv]]%termGen' Hstack]] ; subst ; tea.
+    eapply well_typed_stack_conv_in in Hstack.
+    2: now symmetry.
+    eapply IHπ.
+    2: eassumption.
+    now econstructor.
+Qed.
+
+Lemma well_typed_stack_good Γ A t B (π : stack) :
+  [Γ |- t : A] ->
+  well_typed_stack Γ A t B π ->
+  ∑ π' π'', [× π = π' ++ π'', nomap_stack π' & ismap_stack π''].
+Proof.
+  intros Ht Hty.
+  induction π as [|[]] in A, t, B, Ht, Hty |- *.
+  - exists [::], [::] ; split ; eauto.
+  - eapply well_typed_zip_cons in Hty as [? [? (π'&π''&[])%IHπ]] ; subst ; tea.
+    eexists (eEmptyElim _ :: π'), _ ; split.
+    1: reflexivity.
+    all: eassumption.
+  - eapply well_typed_zip_cons in Hty as [? [? (π'&π''&[])%IHπ]] ; subst ; tea.
+    eexists (eNatElim _ _ _ :: π'), _ ; split.
+    1: reflexivity.
+    all: eassumption.
+  - eapply well_typed_zip_cons in Hty as [? [? (π'&π''&[])%IHπ]] ; subst ; tea.
+    eexists (eApp _ :: π'), _ ; split.
+    1: reflexivity.
+    all: eassumption.
+  - eapply well_typed_zip_cons in Hty as [? [? (π'&π''&[])%IHπ]] ; subst ; tea.
+    eexists (eFst :: π'), _ ; split.
+    1: reflexivity.
+    all: eassumption.
+  - eapply well_typed_zip_cons in Hty as [? [? (π'&π''&[])%IHπ]] ; subst ; tea.
+    eexists (eSnd :: π'), _ ; split.
+    1: reflexivity.
+    all: eassumption.
+  - eexists [::], _ ; split.
+    1-2: reflexivity.
+    pose proof Hty as [? [(?&[->]&?)%termGen' ?]]%well_typed_zip_cons ; tea.
+    eapply list_stack_ismap.
+    2: eapply well_typed_stack_conv_in ; tea.
+    2: now eapply typing_unique.
+    eassumption.
+Qed. *)
 
 Lemma zip_ored t t' π : [t ⇒ t'] -> [zip t π ⇒ zip t' π].
 Proof.
@@ -30,27 +259,76 @@ Proof.
   now eapply zip_ored.
 Qed.
 
-Lemma red_stack_sound :
-  funrect wh_red_stack (fun _ => True) (fun '(t,π) t' => [zip t π ⇒* t']).
+(* Lemma compact_red n π :
+  whne_list n ->
+  ismap_stack π ->
+  [zip n π ⇒* compact n π].
 Proof.
-  intros ? _.
-  funelim (wh_red_stack _).
-  all: cbn; try split; try easy.
-  all: intros v ?.
-  all: etransitivity ; [..|eassumption].
-  all: eapply zip_red.
-  all: econstructor ; [..|reflexivity].
-  all: try now econstructor.
+  intros whn hπ.
+  induction π as [|[] π] in n, whn, hπ |- * ; cbn.
+  1: reflexivity.
+  1-5: cbn in * ; congruence.
+  cbn in * ; fold (ismap_stack π) in hπ.
+  destruct (Map.into_view n) ; cbn.
+  - inversion whn ; subst.
+    + etransitivity.
+      1: now eapply zip_red, redalg_one_step, mapComp.
+      eapply (IHπ (zip1 _ (eMap _ _ _))) ; tea.
+      now econstructor.
+    + inversion H.
+  - eapply (IHπ (zip1 _ (eMap _ _ _))) ; tea.
+    cbn.
+    econstructor.
+    inversion whn ; subst ; tea ; cbn in *.
+    congruence.
 Qed.
 
-Lemma stack_ne n π :
-  whne n -> whne (zip n π).
+Lemma well_typed_compact Γ A t π :
+  whne t ->
+  [Γ |- zip t π : A] ->
+  [zip t π ⇒* compact t π] × whnf (compact t π).
 Proof.
-  intros Hne.
-  induction π as [|[]] in n, Hne |- * ; cbn.
-  1: eassumption.
-  all: eapply IHπ ; now econstructor.
+  intros Hne Hty.
+  apply well_typed_zip in Hty as [? [Ht Hπ]].
+  apply well_typed_stack_good in Hπ as (π'&π''&[-> Hπ' Hπ'']) ; tea.
+  rewrite zip_app, compact_app.
+  unshelve erewrite (stack_compact_nomap _ _ _ Hπ') ; tea.
+  split.
+  1: eapply compact_red ; tea.
+  2: eapply whnf_whne_list, stack_compact_map ; tea.
+  all: econstructor.
+  all: eapply stack_ne ; tea.
+Qed. *)
+
+Section CompactImplSound.
+
+Lemma compact_sound :
+  funrect compact (fun '(b,t,_) => (if b then whne_list t else whne t))
+    (fun '(b,t,π) t' => [zip t π ⇒* t'] × whne_list t').
+Proof.
+  intros ? ?.
+  funelim (compact _).
+  all: cbn ; try easy.
+  2-6: split ; gen_typing.
+  - destruct b.
+    1: easy.
+    split ; [easy|..].
+    now econstructor.
+  - split.
+    1: now econstructor.
+    easy.
+  - inversion H ; subst ; clear H.
+    2: now inversion H0.
+    split.
+    + gen_typing.
+    + intros ? [] ; split ; tea.
+      econstructor ; tea.
+      eapply zip_ored.
+      now econstructor.
 Qed.
+
+Section RedImplemSound.
+
 
 Lemma isType_tm_view1 t e :
   build_tm_view1 t = tm_view1_type e ->
@@ -79,43 +357,100 @@ Proof.
   all: split ; [ now econstructor | intros H' ; inversion H'].
 Qed.
 
-Lemma red_stack_whnf :
-funrect wh_red_stack (fun _ => True) (fun '(t,π) t' => whnf t').
+Lemma red_stack_sound :
+  funrect wh_red_stack (fun _ => True) (fun '(t,π) t' => [zip t π ⇒* t'] × whnf t').
 Proof.
-  intros ? _.
+  intros ? Hty.
   funelim (wh_red_stack _).
-  all: cbn ; try solve [constructor ; eauto]. 
-  - now eapply isType_whnf, isType_tm_view1.
-  - econstructor. eapply stack_ne.
-    now econstructor.
+  all: cbn; try split; try easy.
+  all: match goal with | |- whnf _ => shelve | _ => idtac end.
+  2: shelve.
+  all: intros v [] ; split ; [..|eassumption].
+  all: etransitivity ; [..|eassumption].
+  all: eapply zip_red.
+  1-7: econstructor ; [..|reflexivity] ; now econstructor.
+  now destruct s ; cbn.
+  Unshelve. 
+  - eapply isType_tm_view1 in Heq as [].
+    gen_typing.
+  - now econstructor.
+  - eapply funrect_graph in H ; cycle 1.
+    + eapply compact_sound.
+    + econstructor.
+    + cbn in *.
+      now eapply whnf_whne_list.
   - now eapply whnf_tm_view1_nat.
+  - econstructor.
   - now eapply whnf_tm_view1_list.
+  - eapply funrect_graph in H ; cycle 1.
+    + eapply compact_sound.
+    + econstructor.
+    + now cbn in *.
 Qed.
 
 Corollary _red_sound :
   funrect wh_red (fun _ => True) (fun t t' => [t ⇒* t'] × whnf t').
 Proof.
-  intros ? _.
+  intros ? Hty.
   funelim (wh_red _).
   cbn.
   intros ? H.
-  split.
-  - eapply funrect_graph in H.
-    2: exact red_stack_sound. (* apply fails !? *)
-    all: easy.
-  - eapply funrect_graph in H.
-    2: exact red_stack_whnf.
-    all: easy.
+  eapply funrect_graph in H ; cycle 1.
+  - apply red_stack_sound.
+  - cbn.
+    easy.
+  - eassumption.
 Qed.
+
+(* Lemma can_red_stack :
+  funrect wh_red_stack (fun '(c,π) => isCanonical c × π = [::]) (fun '(c,π) t => c = t).
+Proof.
+  intros ? Hcan.
+  funelim (wh_red_stack _).
+  all: cbn; try split; try easy.
+  all: try solve [destruct Hcan as [] ; congruence].
+  - destruct Hcan as [Hcan _].
+    inversion Hcan.
+  - destruct Hcan as [Hcan _].
+    destruct s ; cbn in *.
+    all: now inversion Hcan.
+  - destruct Hcan as [Hcan _].
+    destruct s ; cbn in *.
+    all: now inversion Hcan.
+Qed.
+
+Lemma can_red c t :
+  isCanonical c ->
+  graph wh_red c t ->
+  t = c.
+Proof.
+  intros Hcan Hgraph.
+  enough (funrect wh_red (fun c => isCanonical c) (fun c t => c = t)).
+  {
+    eapply funrect_graph in Hgraph ; cycle 1 ; tea.
+    cbn in *.
+    now easy.
+  }
+  intros ? ?.
+  funelim (wh_red _).
+  cbn.
+  intros ? Hgraph'.
+  eapply funrect_graph in Hgraph' ; cycle 1.
+  - eapply can_red_stack.
+  - now split.
+  - cbn in *.
+    easy.
+Qed. *)
 
 #[universes(polymorphic)]Corollary red_sound t t' :
   graph wh_red t t' ->
   [t ⇒* t'] × whnf t'.
 Proof.
-  intros H.
-  eapply (funrect_graph wh_red _ _ _ _ _red_sound). (* weird universe inconsistency? *)
-  1: easy.
-  eassumption.
+  intros Hgraph.
+  eapply funrect_graph in Hgraph ; cycle 1.
+  + eapply _red_sound.
+  + easy.
+  + eassumption.
 Qed.
 
 End RedImplemSound.
@@ -161,9 +496,36 @@ Ltac funelim_conv :=
   funelim (conv _); 
     [ funelim (conv_ty _) | funelim (conv_ty_red _) | 
       funelim (conv_tm _) | funelim (conv_tm_red _) | 
-      funelim (conv_ne _) | funelim (conv_ne_red _) ].
+      funelim (conv_ne _) | funelim (conv_ne_red _) |
+      funelim (conv_ne_list _)].
 
 Section ConversionSound.
+
+
+  Lemma whnf_tm_view3_pos T m n :
+    whnf T ->
+    build_nf_view3 T m n = neutrals T m n ->
+    isPosType T.
+  Proof.
+  intros [] ; simp build_nf_view3.
+  all: try solve [congruence].
+  - now econstructor.
+  - now econstructor.
+  - destruct (build_nf_view1 m), (build_nf_view1 n) ; cbn ; try solve [congruence].
+    all: destruct l ; cbn ; try solve [congruence].
+    all: destruct l0 ; cbn ; try solve [congruence].
+  - now econstructor.
+  - destruct (build_ty_view1 n0) ; cbn ; try solve [congruence].
+    + destruct t0 ; cbn ; try solve [congruence].
+      1-2: now econstructor.
+      inversion w ; subst.
+      inversion H.
+    +  destruct n0.
+      1: now do 2 econstructor.
+      destruct s ; cbn in *.
+      all: do 2 econstructor.
+      all: inversion w ; subst ; now inversion H0.
+  Qed.
 
   Import AlgorithmicTypingData.
 
@@ -177,33 +539,16 @@ Section ConversionSound.
   | (ty_state;Γ;_;T;V), (ok _) =>  [Γ |-[al] T ≅ V]
   | (ty_red_state;Γ;_;T;V), (ok _) => [Γ |-[al] T ≅h V]
   | (tm_state;Γ;A;t;u), (ok _) => [Γ |-[al] t ≅ u : A]
-  | (tm_red_state;Γ;A;t;u), (ok _) =>
-      whnf A -> whnf t -> whnf u -> [Γ |-[al] t ≅h u : A]
+  | (tm_red_state;Γ;A;t;u), (ok _) => whnf t -> whnf u -> whnf A -> [Γ |-[al] t ≅h u : A]
   | (ne_state;Γ;_;m;n), (ok T) => [Γ |-[al] m ~ n ▹ T]
   | (ne_red_state;Γ;_;m;n), (ok T) => [Γ |-[al] m ~h n ▹ T] × whnf T
+  | (ne_list_state;Γ;A;m;n), (ok _) => [Γ |-[al] m ~ n :List A]
   end.
-
-  Lemma extract_map_arg_compact t : forall A, extract_map_arg t = (compact_map A t).(Map.lst).
-  Proof. induction t; intros; cbn; reflexivity+ eauto. Qed.
-
-  Lemma is_map_compact_tgtTy {A t} B : is_map t = true ->
-    (compact_map A t).(Map.tgtTy) = (compact_map B t).(Map.tgtTy).
-  Proof.
-    destruct t; cbn; try discriminate; reflexivity.
-  Qed.
-
-  Ltac map_conv_ne := 
-    match goal with 
-    | |- [_ |-[al] ?t ~ ?t' ▹ tList ?C ] =>
-      set (r := compact_map C t);
-      set (r' := compact_map C t');
-      change (tList C) with (tList r.(Map.tgtTy))
-    end; econstructor; cbn.
 
   Lemma _implem_conv_sound :
     funrect conv (fun _ => True) conv_sound_type.
   Proof.
-    intros x _.
+    intros x Hpre.
     funelim_conv ; cbn; try easy.
     all: intros ; simp conv_sound_type; cbn.
     all: match goal with
@@ -223,24 +568,10 @@ Section ConversionSound.
       | s : sort |- _ => destruct s
       end).
     all: try solve [now econstructor].
-    all: try (map_conv_ne ; try rewrite <- extract_map_arg_compact; now cbn).
     - econstructor ; tea.
       now econstructor.
-    - match goal with
-      | |- [ _ |-[al] _ ≅h _ : ?X ] =>
-        match goal with | H : whnf X |- _ => 
-          econstructor ; tea; destruct H ; 
-          simp build_nf_view3 build_ty_view1 in Heq ; 
-          try solve [inversion Heq];
-          econstructor ; tea
-        end
-      end.
-    - match goal with 
-      | |- [_ |-[al] ?t ~ ?t' ▹ tList ?C ] =>
-        set (r := compact_map c t);
-        set (r' := compact_map c t');
-        replace (tList C) with (tList r.(Map.tgtTy))
-      end; econstructor; cbn; repeat rewrite <- extract_map_arg_compact; try now cbn.
+    - econstructor ; tea.
+      now eapply whnf_tm_view3_pos.
     - eapply convne_meta_conv.
       2: reflexivity.
       + econstructor.
@@ -286,7 +617,7 @@ Section TypingCorrect.
     all: inversion 1.
   Qed.
 
-  #[universes(polymorphic)]Definition typing_sound_type
+  #[universes(polymorphic)]Definition typing_sound_post
     (x : ∑ (c : typing_state) (_ : context) (_ : tstate_input c), term)
     (r : result (tstate_output x.π1)) : Type :=
   match x, r with
@@ -299,30 +630,37 @@ Section TypingCorrect.
 
 
   Lemma _implem_typing_sound :
-    funrect typing (fun _ => True) typing_sound_type.
+    funrect typing (fun _ => True) typing_sound_post.
   Proof.
-    intros x _.
+    intros x ?.
     funelim_typing ; cbn.
-    all: intros ; simp typing_sound_type ; try easy ; cbn.
+    all: intros ; simp typing_sound_post ; try easy ; cbn.
     all: repeat (
       match goal with
-      | |- True * _ => split ; [easy|..]
-      | |- forall x : result _, _ => intros [|] ; simp typing_sound_type ; try easy ; cbn
-      | |- _ -> _ => simp typing_sound_type ; intros ?
-      | |- context [match ?t with | _ => _ end] => destruct t ; cbn ; simp typing_sound_type ; try easy
+      | |- _ * _ => split ; [try easy ; shelve |..]
+      | |- forall x : result _, _ => intros [|] ; simp typing_sound_post ; try easy ; cbn
+      | |- _ -> _ => simp typing_sound_post ; intros ?
+      | |- context [match ?t with | _ => _ end] => destruct t ; cbn ; simp typing_sound_post ; try easy
       | s : sort |- _ => destruct s
-      | H : graph wh_red _ _ |- _ => eapply red_sound in H as []
-      | H : graph conv _ _ |- _ => eapply implem_conv_sound in H ; simp conv_sound_type in H
+      | H : graph wh_red _ _ |- _ => shelve
+      | H : graph conv _ _ |- _ => shelve
       | H : ctx_access _ _ = _ |- _ => eapply ctx_access_correct in H
       | H : (build_ty_view1 _ = ty_view1_small _) |- _ => eapply ty_view1_small_can in H
       | H : (_;_;_) = (_;_;_) |- _ => injection H; clear H; intros; subst 
       end).
     all: now econstructor.
+    Unshelve.
+    - injection eqargs ; clear eqargs ; intros ; subst.
+      eapply implem_conv_sound in H ; cbn in *.
+      1: now econstructor.
+    - injection eqargs ; clear eqargs ; intros ; subst.
+      eapply red_sound in H as [].
+      1: now econstructor.
   Qed.
 
   Lemma implem_typing_sound x r:
     graph typing x r ->
-    typing_sound_type x r.
+    typing_sound_post x r.
   Proof.
     eapply funrect_graph.
     1: now apply _implem_typing_sound.
